okasaki/BootstrappedQueue_proof.v
@@ -3,24 +3,6 @@ Require Import FuncTactics LibCore.
 Require Import QueueSig_ml QueueSig_proof.
 Require Import BootstrappedQueue_ml.
 
-Lemma list_rep_cons : forall `{Rep a A} l L x X,
-  rep l L -> rep x X -> rep (x::l) (X::L).
-Proof. intros. constructors~. Qed.
-Hint Resolve @list_rep_cons.
-
-Lemma cons_neq_nil : forall A (x:A) l, x::l <> nil.
-Proof. auto_false. Qed.
-Hint Immediate cons_neq_nil.
-
-Hint Constructors Forall2.
-Hint Resolve Forall2_last.
-Lemma Forall2_rev : forall A1 A2 (P:A1->A2->Prop) l1 l2,
-  Forall2 P l1 l2 -> Forall2 P (rev l1) (rev l2).
-Proof. induction l1; introv M; inverts M; rew_rev; auto. Qed.
-
-
-
-
 Module BootstrappedQueueSpec <: QueueSigSpec.
 
 (** instantiations *)
@@ -70,20 +52,19 @@ Defined.
 
 Hint Constructors doubling inv Forall2.
 Hint Resolve Forall2_last Forall2_rev.
+Hint Immediate cons_neq_nil.
 Ltac auto_tilde ::= eauto with maths.
 Hint Extern 1 (@gt nat _ _ _) => simpl; math.
 
 (** useful facts *)
 
-Fixpoint depth a (q:queue a) : nat :=
-  match q with
-  | Empty => 0%nat
-  | Struct lenfm f m lenr r => (1 + depth m)%nat
-  end.
-
 Coercion queue_of_body a (q:body a) : queue a :=
   let '(lenfm,f,m,lenr,r) := q in
   Struct lenfm f m lenr r.
+
+Definition is_empty_front a (q:body a) : bool :=
+  let '(lenfm,f,m,lenr,r) := q in
+  match f with nil => true | _ => false end.
 
 Lemma to_empty : forall `{Rep a A} Q,
   rep Empty Q -> Q = nil.
@@ -140,32 +121,6 @@ Proof.
    forwards~: IHD. maths (2*n>=1). lets~: (IHD H0).
 Qed.
 
-(* todo: check needed *)
-
-Lemma decrease_r : forall A (Q Qf Qm Qr : list A) Qms,
-  Q = Qf ++ Qm ++ rev Qr ->
-  0 < length Qr -> 
-  Qm = concat Qms ->
-  doubling true 1 Qms ->
-  length Qms < length Q.
-Proof.
-  introv E L Em Dm. destruct Qr. gen L. rew_list~. 
-  forwards: (concat_doubling_length Dm).
-  subst Q Qm. rew_length~.
-Qed.
-
-Lemma decrease_f : forall `{Rep a A} f (Q Qf Qm Qr : list A) Qms,
-  Q = Qf ++ Qm ++ rev Qr ->
-  f <> nil -> rep f Qf ->
-  Qm = concat Qms ->
-  doubling true 1 Qms ->
-  length Qms < length Q.
-Proof.
-  introv E L R Em Dm. destruct f. false. inverts R.
-  forwards: (concat_doubling_length Dm).
-  subst Q Qm. rew_length~.
-Qed.
-
 (** verification *)
 
 Lemma empty_spec : forall `{Rep a A},
@@ -192,40 +147,40 @@ Hint Extern 1 (RegisterSpec is_empty) => Provide is_empty_spec.
 
 Definition checkq_specs `{Rep a A} :=
   Spec checkq (q:body a) |R>>
-     forall Q, inv false false q Q -> R (Q ;- queue a).
+    forall Q, inv false false q Q -> R (Q ;- queue a).
 
 Definition checkf_specs `{Rep a A} :=
   Spec checkf (q:body a) |R>>
-     forall Q, inv true false q Q -> R (Q ;- queue a).
+    forall Q, inv true false q Q -> R (Q ;- queue a).
 
-Definition snoc_specs_aux `{Rep a A} :=
-  Spec snoc (q:queue a) (x:a)|R>>
-     forall X Q, rep x X -> rep q Q ->
-     R (fun q' => rep q' (Q&X) 
-        /\ (q <> Empty -> depth q' = depth q)
-        /\ (q = Empty -> q' = Struct 1 (x::nil) Empty 0 nil)).
+Definition snoc_specs `{Rep a A} :=
+  RepTotal snoc (Q;queue a) (X;a) >> (Q & X) ;- queue a.
+
 Definition head_specs `{Rep a A} :=
   RepSpec head (Q;queue a) |R>>
-     Q <> nil -> R (is_head Q ;; a).
+    Q <> nil -> R (is_head Q ;; a).
 
 Definition tail_specs `{Rep a A} :=
   RepSpec tail (Q;queue a) |R>> 
-     Q <> nil -> R (is_tail Q ;; queue a).
+    Q <> nil -> R (is_tail Q ;; queue a).
 
 Lemma all_specs : 
   (forall `{Rep a A}, checkq_specs) /\ 
   (forall `{Rep a A}, checkf_specs) /\ 
-  (forall `{Rep a A}, snoc_specs_aux) /\
+  (forall `{Rep a A}, snoc_specs) /\
   (forall `{Rep a A}, head_specs) /\
   (forall `{Rep a A}, tail_specs).
-(*
 Proof.
   eapply conj_strengthen_5; try intros M; intros; try (unfolds; xintros).
-  intros q. intros. gen_eq n:((3 * depth q + 1)%nat). gen n a A q Q H0. apply M.
-  intros q. intros. gen_eq n:((3 * depth q)%nat). gen n a A q Q H0. apply M.
-  intros q x. intros. gen_eq n:((3 * depth q + 2)%nat). gen n a A q x Q X H0 H1. apply M.
+  intros q. intros. gen_eq n:((if is_empty_front q 
+    then 3 * length Q + 3 else 3 * length Q - 2)%nat).
+    gen n a A q Q H0. apply M.
+  intros q. intros. gen_eq n:(if is_empty_front q 
+    then (3 * length Q + 2)%nat else 0%nat).
+    gen n a A q Q H0. apply M.
+  intros q x. intros. gen_eq n:((3 * length Q + 2)%nat). gen n a A q x Q X H0 H1. apply M.
   intros q. intros. gen_eq n:(0%nat). gen n a A q Q H0 H1. apply M.
-  intros q. intros. gen_eq n:((3 * depth q + 2)%nat). gen n a A q Q H0 H1. apply M.
+  intros q. intros. gen_eq n:((3 * length Q + 1)%nat). gen n a A q Q H0 H1. apply M.
   forwards (H1&H2&H3&H4&H5): (eq_gt_induction_5);
     try match goal with |- _ /\ _ /\ _ /\ _ /\ _ =>
       splits; intros n; pattern (eq n);
@@ -233,38 +188,23 @@ Proof.
     auto~.
   introv IHcheckq IHcheckf IHsnoc IHhead IHtail. simpls. splits.
   (* verification of checkq *)
-  clear IHcheckq IHtail.
-  introv RQ N. subst n. xcf_app. xmatch. xif.
-  inverts RQ. subst q. xapp. constructors~. auto~.
-  inverts RQ. subst q. (* ? xapp (>>> (list a) Qms (rev Qr)). *)
-  specializes IHsnoc (>>> (list a) Qms (rev Qr)). xapp~. simpls.
-  destruct P_x3 as (P3&PN3&PE3).
-  destruct (classic (m = Empty)). 
-    (* case empty *)
-    clear PN3 IHsnoc. subst m Qm. inverts H11. 
-    rew_concat in *. rew_length in H18. 
-    apply app_spec_1. apply~ checkf_cf. xisspec.
-    intros b B. subst b. xmatch. xmatch.
-      xret. inverts H9. inverts P3.
-      specializes IHhead (>>> (list a) (rev Qr :: nil)). xapp~. clear IHhead.
-      xlet (= Empty (A:=list a)). apply app_spec_1. apply~ tail_cf. xisspec.
-       intros b B. subst b. rewrite~ PE3. xmatch.
-      apply app_spec_1. apply~ checkq_cf. xisspec.
-       intros b B. subst b. xmatch. xif; try math.
-      apply app_spec_1. apply~ checkf_cf. xisspec.
-       intros b B. subst b q. xmatch. xmatch. xret~. false~ C3.
-      subst _x0. xret. xrep in P_x2. inverts H9. subst Q.
-       rew_list. rew_length in *. inverts PX as M. inverts M.
-         constructors~. rew_length~. rew_list~. simpl in RX.
-         intro_subst_hyp. inverts RX as M. applys_to M nil_eq_rev_inv.
-          subst Qr. rew_length in *. math.
-      xret. constructors~. rew_list~. rew_list~. intro_subst_hyp. false~ C1.
-       apply~ doubling_cons. rew_length~.
-    (* case not empty *)
-    clear PE3 IHhead. 
-    xapp. constructors~. subst Qm. rew_list~. subst Q Qm. rew_list~.
-    apply~ doubling_last. subst Qm. rew_length~.
-    simpl. rewrite~ PN3.
+  clear IHcheckq IHhead IHtail.
+  introv RQ N. subst n. xcf_app. xmatch; inverts RQ.
+  rename H9 into RQf. xif.
+  subst q. xapp. constructors~. simpl. destruct f.
+    math. 
+    inverts RQf. subst Q. rew_list~.
+  forwards~: (@concat_doubling_length _ Qms).
+   specializes IHsnoc (>>> (list a) Qms (rev Qr)). xapp~; clear IHsnoc.
+     destruct f; simpl.
+       subst Q Qm. rew_list~.
+       inverts RQf. subst Q Qm. rew_list~.
+   simpls. xapp~.
+     constructors~.
+       subst. rew_list~.
+       subst. rew_list~.
+       apply~ doubling_last. subst Qm. rew_length~.
+     destruct f; simpl. math. inverts RQf. subst Q. rew_length~. 
   (* verification of checkf *)
   clear IHcheckq IHcheckf IHsnoc.
   introv RQ N. subst n. xcf_app. xmatch. xmatch.
@@ -273,63 +213,47 @@ Proof.
     forwards~ M: (@length_zero_inv _ Qr). subst Qr. 
     inverts RR. subst Q. rew_list. constructors~.
   inverts RQ. inverts H9. 
-  specializes IHhead (>>> (list a) Qms). xapp~. clear IHhead.
-   intro_subst_hyp. applys C. fequals. apply~ @from_empty.
-  destruct P_x2 as (Hm'&RHm'&[Tm' EQms']). 
-  specializes IHtail (>>> (list a) Qms). xapp~. clear IHtail.
-  destruct P_x3 as (Tm&RHm&[Hm EQms]). 
-  subst Qms. injects EQms. subst Q Qm. xgo.
-  rew_list in H18. inverts H22 as K P. constructors~. rew_list~.
-   intro_subst_hyp. inverts RHm'. rew_list in P. math.
-   apply~ doubling_weaken_f.
+   specializes IHhead (>>> (list a) Qms). xapp~. 
+    intro_subst_hyp. applys C. fequals. apply~ @from_empty.
+   clear IHhead. destruct P_x2 as (Hm'&RHm'&[Tm' EQms']). 
+   specializes IHtail (>>> (list a) Qms). xapp~.
+    simpl. subst Q Qm. rew_length. 
+    forwards~: (@concat_doubling_length _ Qms).
+   clear IHtail. destruct P_x3 as (Tm&RHm&[Hm EQms]). 
+   subst Qms. injects EQms. subst Q Qm. xgo.
+   rew_list in H18. inverts H22 as K P. constructors~. rew_list~.
+    intro_subst_hyp. inverts RHm'. rew_list in P. math.
+    apply~ doubling_weaken_f.
   xgo. inverts RQ. constructors~. intro_subst_hyp. inverts H10. false~ C0.
   (* verification of snoc *)
   clear IHcheckf IHsnoc IHhead IHtail.
-  introv RX RQ N. subst n. xcf_app. xgo.
-  inverts RQ. splits; auto_false. constructors~.
-  inverts RQ. 
-  specializes IHcheckq a __ __. eapply app_weaken_1.
-  fapplys IHcheckq. constructors~. rew_list~. simple~.
-   ximpl as q'. subst Q. splits; auto_false.
-     applys_eq Hx 1. rew_list~.
-     introv K. simpl.
-xapp~. clear IHtail.
-xapp~. constructors~. rew_list~. subst. rew_list~.
-  rew_length~.
+  introv RQ RX N. subst n. xcf_app. inverts RQ; xgo.
+  constructors~.
+  constructors~. rew_length~. subst Q. rew_list~.
+  simpl. destruct f. false. rew_length~.
   (* verification of head *)
   clear IHcheckf IHcheckq IHsnoc IHhead IHtail.
-  introv RQ NE N. subst n. xcf_app. xgo.
-  inverts RQ. false.
-  inverts RQ. inverts~ H9.
-  inverts RQ. false. destruct f; false.
+  introv RQ NE N. subst n. xcf_app. inverts RQ. false. 
+  xgo. inverts~ H4. destruct f; false.
   (* verification of tail *)
   clear IHcheckf IHsnoc IHhead IHtail.
-  introv RQ RX N. subst n. xcf_app. xmatch.
-  xgo. inverts RQ. false.
-  inverts RQ. inverts H9. specializes IHcheckq a (l2 ++ Qm ++ rev Qr).
-  xapp. clear IHcheckq.
-   constructors~. subst. rew_list~.
-  auto~.
-  ximpl~.
-  xgo. inverts RQ. false. destruct f; false.
+  introv RQ RX N. subst n. xcf_app. inverts RQ. false. xmatch.
+  inverts H4. specializes IHcheckq a (l2 ++ Qm ++ rev Qr).
+   xapp; clear IHcheckq.
+     constructors~. subst. rew_list~.
+     simpl. subst Q. rew_length. destruct f'; math.
+     ximpl~.
+  xgo. destruct f; false.
 Qed.
 
-*)
-Admitted.
+Lemma head_spec : forall `{Rep a A}, head_specs.
+Proof. intros. apply~ (proj54 all_specs). Qed.
 
-Definition snoc_specs `{Rep a A} :=
-  RepTotal snoc (Q;queue a) (X;a) >> (Q & X) ;- queue a.
+Lemma tail_spec : forall `{Rep a A}, tail_specs.
+Proof. intros. apply~ (proj55 all_specs). Qed.
 
-
-(*
-Definition head_spec := proj53 all_specs.
-Definition tail_spec := proj54 all_specs.
-Definition snoc_spec := proj55 all_specs.
-*)
-
-Axiom head_spec : forall `{Rep a A}, head_specs.
-Axiom tail_spec : forall `{Rep a A}, tail_specs.
-Axiom snoc_spec : forall `{Rep a A}, snoc_specs.
+Lemma snoc_spec : forall `{Rep a A}, snoc_specs.
+Proof. intros. apply~ (proj53 all_specs). Qed.
 
 Hint Extern 1 (RegisterSpec head) => Provide head_spec.
 Hint Extern 1 (RegisterSpec tail) => Provide tail_spec.
